

# Representation Theory

## Homework 5

Ari Feiglin

### 1 Problem

Let  $V$  be an  $\mathbb{F}$ -vector space, and define  $\text{end}_{\mathbb{F}}^{\text{frk}}(V) \subseteq \text{end}_{\mathbb{F}}(V)$  be the set of all finite-rank  $V$ -endomorphisms (endomorphisms whose image is finite-dimensional).

- (1) Show that for  $T \in \text{end}_{\mathbb{F}}^{\text{frk}}(V)$ ,  $TV$  is  $T$ -invariant and as such we can define  $\text{tr}_V(T) = \text{tr}_{TV}(T)$ . Show that  $\text{tr}: \text{end}_{\mathbb{F}}^{\text{frk}}(V) \rightarrow \mathbb{F}$  is linear.
- (2) Show that  $\text{tr}: \text{end}_{\mathbb{F}}^{\text{frk}}(V) \rightarrow \mathbb{F}$  decomposes as the composition  $\text{end}_{\mathbb{F}}^{\text{frk}}(V) \cong V^{\vee} \otimes_{\mathbb{F}} V \xrightarrow{\text{ev}} \mathbb{F}$ , where the first map is the standard isomorphism, and the second is induced by the bilinear map  $V^{\vee} \times V \rightarrow \mathbb{F}, (\phi, v) \mapsto \phi(v)$ .

- (1) For any  $V$ -endomorphism,  $TV$  is  $T$ -invariant, as such  $\text{tr}$  is clearly well-defined. Note that if  $TV \subseteq W$  is also finite-dimensional then  $\text{tr}_{TV}(T) = \text{tr}_W(T)$ . Indeed: take  $B = \{v_1, \dots, v_n\}$  to be a basis for  $TV$  and extend it to a basis  $B' = \{v_1, \dots, v_n, v_{n+1}, \dots, v_m\}$  of  $W$ . Then we have

$$\text{tr}_{TV}(T) = \sum_{i=1}^n ([Tv_i]_B)_i$$

and

$$\text{tr}_W(T) = \sum_{i=1}^m ([Tv_i]_{B'})_i$$

Now, for  $1 \leq i \leq n$ , notice that  $Tv_i \in \text{span}\{v_1, \dots, v_n\}$  and as such  $[Tv_i]_{B'}$  is equal to  $[Tv_i]_B$  but with  $m - n$  padded zeroes. Thus,  $([Tv_i]_{B'})_i = ([Tv_i]_B)_i$ . And for  $i > n$ ,  $Tv_i \in TV = \text{span}\{v_1, \dots, v_n\}$ , so in the linear combination of basis vectors equalling  $Tv_i$ , the coefficients of  $v_{n+1}, \dots, v_m$  are zero. In particular,  $([Tv_i]_{B'})_i = 0$ . So we have

$$\text{tr}_W(T) = \sum_{i=1}^n ([Tv_i]_B)_i = \text{tr}_{TV}(T)$$

Now, notice that for  $T, S \in \text{end}_{\mathbb{F}}^{\text{frk}}(V)$ , we have  $(T + S)V, TV, SV \subseteq TV + SV$  (which is finite-dimensional) and so

$$\text{tr}(T+S) = \text{tr}_{(T+S)V}(T+S) = \text{tr}_{TV+SV}(T+S) = \text{tr}_{TV+SV}(T) + \text{tr}_{TV+SV}(S) = \text{tr}_{TV}(T) + \text{tr}_{SV}(S) = \text{tr}(T) + \text{tr}(S)$$

And similarly  $(\alpha T)V \subseteq TV$  so

$$\text{tr}(\alpha T) = \text{tr}_{(\alpha T)V}(\alpha T) = \text{tr}_{TV}(\alpha T) = \alpha \text{tr}(T)$$

So  $\text{tr}$  is indeed linear.

- (2) We recall the isomorphism  $V^{\vee} \otimes_{\mathbb{F}} V \cong \text{end}_{\mathbb{F}}^{\text{frk}}(V)$ , induced by mapping  $(\phi, v) \mapsto [u \mapsto \phi(u)v]$ . Its inverse, recall is given as follows: for  $T \in \text{end}_{\mathbb{F}}^{\text{frk}}(V)$ , let  $\{e_1, \dots, e_n\}$  be a basis for  $TV$ . Then define  $\pi_i: V \rightarrow \mathbb{F}$  by extending the  $i$ th projection of  $TV \rightarrow \mathbb{F}$  to all of  $V$ . Then the image of  $T$  is

$$\sum_{i=1}^n (\pi_i \circ T) \otimes e_i$$

Now, we know that  $\text{ev}: V^\vee \otimes_{\mathbb{F}} V \rightarrow \mathbb{F}$  by  $\text{ev}(\phi \otimes v) \mapsto \phi(v)$ . As such

$$\sum_{i=1}^n (\pi_i \circ T) \otimes e_i \mapsto \sum_{i=1}^n \pi_i(Te_i) = \text{tr}(T)$$

(Since  $\pi_i(Te_i) = ([Te_i]_B)_i$ ).

## 2 Problem

Let  $V$  be a  $G$ -representation and  $W$  an  $H$ -representation. Show that there is an equivariant  $G \times H$  injection  $V^\vee \otimes_{\mathbb{F}} W^\vee \rightarrow (V \otimes_{\mathbb{F}} W)^\vee$ . Show that if either  $V$  or  $W$  are finite-dimensional then this is an isomorphism.

We begin by defining a  $G \times H$ -equivariant bilinear map  $V^\vee \times W^\vee \rightarrow (V \otimes_{\mathbb{F}} W)^\vee$ , and this will induce a  $G \times H$ -equivariant map from the tensor product. Given  $\lambda, \mu \in V^\vee \times W^\vee$ , define  $f(\lambda, \mu): V \otimes W \rightarrow \mathbb{F}$  by  $f(\lambda, \mu)(v, w) = \lambda(v)\mu(w)$ . This is clearly a bilinear map, and as such defines a map (abusing notation by recycling the name)  $f(\lambda, \mu): V \otimes_{\mathbb{F}} W \rightarrow \mathbb{F}$ , i.e.  $f(\lambda, \mu) \in (V \otimes_{\mathbb{F}} W)^\vee$ . This map  $f: V^\vee \times W^\vee \rightarrow (V \otimes_{\mathbb{F}} W)^\vee$  is bilinear as well:

$$f(\lambda + \lambda', \mu)(v \otimes w) = (\lambda + \lambda')(v)\mu(w) = (f(\lambda, \mu) + f(\lambda', \mu))(v \otimes w)$$

etc. As such it defines a map  $f: V^\vee \otimes W^\vee \rightarrow (V \otimes_{\mathbb{F}} W)^\vee$ , explicitly given by

$$f(\lambda \otimes \mu)(v \otimes w) = \lambda(v)\mu(w)$$

(The work we have done thus far is to show that this is well-defined.)

Now we claim two things: that  $f$  is  $G \times H$ -equivariant, and that  $f$  is an injection. First, note that for  $g, h \in G \times H$ :

$$f((g, h)\lambda \otimes \mu)(v \otimes w) = f((g\lambda) \otimes (h\mu))(v \otimes w) = (g\lambda)(v) \cdot (h\mu)(w) = \lambda(g^{-1}v)\mu(h^{-1}w)$$

We now consider the action of  $G \times H$  on  $(V \otimes_{\mathbb{F}} W)^\vee$ : given  $\phi \in (V \otimes_{\mathbb{F}} W)^\vee$  and  $g, h \in G \times H$ :

$$(g, h) \star \phi: (v \otimes w) \mapsto \phi((g, h)^{-1}(v \otimes w)) = \phi((g^{-1}, h^{-1})(v \otimes w)) = \phi((g^{-1}v) \otimes (h^{-1}w))$$

As such,

$$(g, h)f(\lambda \otimes \mu): (v \otimes w) \mapsto f(\lambda \otimes \mu)(g^{-1}v \otimes h^{-1}w) = \lambda(g^{-1}v)\mu(h^{-1}w)$$

By linearity this holds for all  $\phi \in V^\vee \otimes W^\vee$ . Thus we have indeed that

$$f((g, h)\bullet) = (g, h)f(\bullet)$$

as required.

Now, to show that  $f$  is injective. Let  $\{\lambda_i\}_{i \in I}$  be a basis for  $V^\vee$ , then elements of  $V^\vee \otimes W^\vee$  are of the form  $\sum_{i \in I} \lambda_i \otimes \phi_i$  for  $\phi_i \in W^\vee$ , all but finitely many being zero. Now, if  $x = \sum_{i \in I} \lambda_i \otimes \phi_i \neq 0$ , we claim that its image is also nonzero (and so  $f$  has a trivial kernel, making it injective). Indeed, since it is nonzero there is some  $i_0 \in I$  with  $\phi_{i_0} \neq 0$ . As such, suppose  $\phi_{i_0}(w) \neq 0$ . Let us define  $\psi \in V^\vee$  by  $\psi(v) = \sum_{i \in I} \lambda_i(v)\phi_i(w)$ , i.e.  $\psi(v) = f(x)(v, w)$ . Now, we have

$$\psi = \sum_{i \in I} \lambda_i \cdot \phi_i(w)$$

i.e.  $\psi$  is a linear combination of  $\lambda_i$ s. Since  $\lambda_i$  forms a basis for  $V^\vee$ , and a coefficient  $(\phi_{i_0}(w))$  is nonzero, we must have that  $\psi \neq 0$ . In particular, this means that  $f(x) \neq 0$ , as desired.

If  $V$  or  $W$  are finite-dimensional, we claim that this is a surjection as well. Without loss of generality, assume  $V$  is finitely generated, with a basis  $\{e_1, \dots, e_n\}$  and dual basis  $\{e_1^*, \dots, e_n^*\}$ . Now let  $\phi \in (V \otimes_{\mathbb{F}} W)^{\vee}$ . Let us define  $\phi_j \in W^{\vee}$  by  $\phi_j(w) = \phi(e_j \otimes w)$ . This is clearly linear. Furthermore, notice that

$$\phi(v \otimes w) = \phi\left(\sum_{i=1}^n e_i^*(v) e_i \otimes w\right) = \sum_{i=1}^n e_i^*(v) \phi(e_i \otimes w) = \sum_{i=1}^n e_i^*(v) \phi_i(w)$$

Thus

$$\phi(v \otimes w) = f\left(\sum_{i=1}^n e_i^* \otimes \phi_i\right)(v \otimes w) \implies \phi = f\left(\sum_{i=1}^n e_i^* \otimes \phi_i\right)$$

as required.

### 3 Problem

Let  $V$  be a vector space over a field of characteristic  $\neq 2$ . Define

$$\text{Sym}^2 V = \text{span}\{v_1 \otimes v_2 + v_2 \otimes v_1\}, \quad \Lambda^2 V = \text{span}\{v_1 \otimes v_2 - v_2 \otimes v_1\} \subseteq V \otimes_{\mathbb{F}} V$$

- (1) Show that  $V \otimes_{\mathbb{F}} V = \text{Sym}^2 V \oplus \Lambda^2 V$ ;
- (2) Given  $n = \dim V$ , compute  $\dim \text{Sym}^2 V, \dim \Lambda^2 V$ ;
- (3)  $S_2$  acts naturally on  $V \otimes_{\mathbb{F}} V$ . Show that  $\text{Sym}^2 V, \Lambda^2 V$  are subrepresentations. How does  $S_2$  act on each?
- (4) Assume that  $V$  is a  $G$ -representation. Show that  $\text{Sym}^2 V, \Lambda^2 V \subseteq V \otimes_{\mathbb{F}} V$  are subrepresentations. Deduce that if  $\dim V > 1$ ,  $V \otimes_{\mathbb{F}} V$  is not irreducible.

- (1) Let us define an endomorphism of  $V \otimes V$ , namely

$$f(v \otimes w) = \frac{v \otimes w + w \otimes v}{2}$$

This is induced by the bilinear function  $f(v, w) = \frac{v \otimes w + w \otimes v}{2}$ , and as such is well-defined. Clearly, the image of  $f$  is  $\text{Sym}^2 V$ : it is clear that  $f(v \otimes w) \in \text{Sym}^2 V$ , and as such  $\text{im } f \subseteq \text{Sym}^2 V$ . Conversely,  $\text{Sym}^2 V$  is spanned by  $\frac{v \otimes w + w \otimes v}{2}$ , i.e. elements of the form  $f(v \otimes w)$ . Also,  $f$  is idempotent: since  $f(v \otimes w) = f(w \otimes v)$ ,

$$f^2(v \otimes w) = \frac{f(v \otimes w) + f(w \otimes v)}{2} = f(v \otimes w)$$

Thus  $f$  is a projection operator onto  $\text{Sym}^2 V$ . So we have  $V \otimes_{\mathbb{F}} V = \text{Sym}^2 V \oplus \ker f$ . Notice that since  $f(v \otimes w) = f(w \otimes v)$ , we have  $\Lambda^2 V \subseteq \ker f$ .

Let us also define

$$g(v \otimes w) = \frac{v \otimes w - w \otimes v}{2}$$

Which is again well-defined, and a projection onto  $\Lambda^2 V$ . But notice that  $f + g = \text{id}$ .

As such, if  $v \in \ker f$  then  $v = f v + g v = g v \in \Lambda^2 V$ . Thus,  $\ker f = \Lambda^2 V$ . So we have shown

$$V \otimes_{\mathbb{F}} V = \text{Sym}^2 V \oplus \Lambda^2 V$$

as required.

- (2) Let  $B = \{e_i\}_{i=1}^n$  be a basis for  $V$ . Then  $B_2 = \{e_i \otimes e_j\}$  is a basis for  $V \otimes_{\mathbb{F}} V$ , and in particular we have  $\dim V \otimes_{\mathbb{F}} V = n^2$ . Since  $f, g$  are projection operators into  $\text{Sym}^2 V$  and  $\Lambda^2 V$  respectively,  $fB_2, gB_2$  form bases for  $\text{Sym}^2, \Lambda^2 V$  respectively. Now, notice that since  $f(e_i \otimes e_j) = f(e_j \otimes e_i)$ ,

$$\text{Sym}^2 V = \text{span} f(B_2) = \text{span} \{f(e_i \otimes e_j)\}_{i,j} = \text{span} \{f(e_i \otimes e_j)\}_{i \leq j}$$

and similarly since  $g(e_i \otimes e_j) = -g(e_j \otimes e_i)$  (and in particular  $g(v \otimes v) = 0$ ),

$$\Lambda^2 V = \text{span} g(B_2) = \text{span} \{f(e_i \otimes e_j)\}_{i < j}$$

In particular, we have  $\dim \text{Sym}^2 V \leq \binom{n}{2} + n = \frac{n(n+1)}{2}$  and  $\dim \Lambda^2 V \leq \binom{n}{2} = \frac{n(n-1)}{2}$  (as these are the number of ways of choosing  $i \leq j$  and  $i < j$  respectively). Now, notice that since  $V \otimes V = \text{Sym}^2 V \oplus \Lambda^2 V$ , we have

$$\dim V \otimes V = n^2 = \dim \text{Sym}^2 V + \dim \Lambda^2 V \leq \frac{n(n+1)}{2} + \frac{n(n-1)}{2} = n^2$$

As such, these inequalities must be equalities, and we have

$$\dim \text{Sym}^2 V = \frac{n(n+1)}{2}, \quad \dim \Lambda^2 V = \frac{n(n-1)}{2}$$

- (3)  $S_2$  acts on  $V \otimes V$  by  $\sigma(v_1 \otimes v_2) = v_{\sigma 1} \otimes v_{\sigma 2}$ . The only non-trivial element of  $S_2$  is  $\sigma = (1\ 2)$ , so this can be simplified to  $(1\ 2)(v \otimes u) = u \otimes v$ .

On  $\text{Sym}^2 V$ , note that for  $v \otimes u + u \otimes v$ ,  $\sigma(v \otimes u + u \otimes v) = u \otimes v + v \otimes u$ . So  $\sigma$  acts trivially on the generators of  $\text{Sym}^2 V$  (as such it is a subrepresentation), and thus on all of  $\text{Sym}^2 V$ . So  $S_2$  acts trivially on  $\text{Sym}^2 V$ .

On  $\Lambda^2 V$  we have  $\sigma(v \otimes u - u \otimes v) = u \otimes v - v \otimes u$ . So  $\sigma$  acts as multiplication by  $-1$  on  $\Lambda^2 V$  (and as such it is a subrepresentation).

- (4) We will show that  $f, g$  (defined above) are  $G$ -equivariant. Indeed, let us define  $s: V \otimes V \rightarrow V \otimes V$  by  $v \otimes u \mapsto u \otimes v$ . Then

$$f = \frac{\text{id} + s}{2}, \quad g = \frac{\text{id} - s}{2}$$

So we just need to show that  $s$  is  $G$ -equivariant, and then by linearity so to are  $f, g$ .

Indeed, let  $h \in G$ , then

$$s(h(v \otimes u)) = s((hv) \otimes (hu)) = (hu) \otimes (hv) = h(u \otimes v) = h(s(v \otimes u))$$

as required.

Since  $f, g$  are  $G$ -equivariant, their images are  $G$ -subrepresentations. These images are the subspaces  $\text{Sym}^2 V, \Lambda^2 V$ , and so we have shown the desired result.

Now, if  $n = \dim V > 1$ , we have that  $\frac{n(n+1)}{2}, \frac{n(n-1)}{2} < n^2$ . As such, by considering dimensions,  $\text{Sym}^2 V, \Lambda^2 V$  are proper (nontrivial) subspaces of  $V \otimes V$ . Therefore  $V \otimes V$  cannot be simple.

#### 4 Problem

Let  $V$  be a  $G$ -representation over a field with characteristic  $\neq 2$ .

- (1) Identify bilinear forms on  $V$  with elements in  $\text{hom}_{\mathbb{F}}(V \otimes V, \mathbb{F})$ . Show that a form is  $G$ -invariant iff it is in  $\text{hom}_G(V \otimes V, \mathbb{F})$ .

- (2) Show that a map  $V \otimes V \rightarrow \mathbb{F}$  factors as a composition  $V \otimes V \xrightarrow{p_1} \text{Sym}^2 V \rightarrow \mathbb{F}$  iff it corresponds to a symmetric form, and  $V \otimes V \xrightarrow{p_2} \Lambda^2 V \rightarrow \mathbb{F}$  iff it corresponds to an antisymmetric form.

- (1) Let  $(\bullet, \bullet)$  be a bilinear form. Then it corresponds to the map  $f \in (V \otimes V)^\vee$  given by  $f(v \otimes w) = (v, w)$ . We claim that  $(\bullet, \bullet)$  is  $G$ -invariant iff  $f$  is  $G$ -equivariant (note that  $\mathbb{F}$  is trivial, so  $f$  being equivariant means  $f(gx) = f(x)$ ). Indeed:

$$f(g(v \otimes w)) = f((gv) \otimes (gw)) = (gv, gw)$$

So  $(gv, gw) = (v, w)$  iff  $f(g(v \otimes w)) = f(v \otimes w)$ . This means that if  $(\bullet, \bullet)$  is  $G$ -invariant, then  $f$  is  $G$ -equivariant (since it satisfies  $f(gx) = f(x)$  for generators  $x$ , by linearity this extends to all  $x$ ). And conversely if  $f$  is  $G$ -equivariant, then the bilinear form is  $G$ -invariant.

Thus  $(\bullet, \bullet)$  is  $G$ -invariant iff  $f \in \text{hom}_G(V \otimes V, \mathbb{F})$  (i.e. it corresponds to an element in  $\text{hom}_G(V \otimes V, \mathbb{F})$ ).

- (2) Notice that  $p_1(v \otimes u) = p_1(u \otimes v)$  (as  $v \otimes u - u \otimes v \in \Lambda^2 V$ , which is the complement of  $\text{Sym}^2 V$ ). As such a map  $f: V \otimes V \xrightarrow{p_1} \text{Sym}^2 V \xrightarrow{q_1} \mathbb{F}$  satisfies  $f(v \otimes u) = q_1 p_1(v \otimes u) = q_1 p_1(u \otimes v) = f(u \otimes v)$ . Thus  $f$  corresponds to a symmetric bilinear form.

Similarly,  $p_2(v \otimes u) = -p_2(u \otimes v)$ . Thus  $f(v \otimes u) = q_2 p_2(v \otimes u) = -q_2 p_2(u \otimes v) = -f(u \otimes v)$ , so  $f$  corresponds to an antisymmetric bilinear form.

Now, if  $(\bullet, \bullet)$  is a symmetric bilinear form, then let it correspond to  $f: V \otimes V \rightarrow \mathbb{F}$ . We need to show that if  $p_1(v \otimes u) = p_1(z \otimes w)$  then  $(v, u) = (z, w)$  (since then  $q_1(p_1(v \otimes u)) = (v, u)$  will be well-defined, and extends by linearity to satisfy our demand). Indeed,  $v \otimes u - z \otimes w \in \ker p_1 = \Lambda^2 V$ . Since  $(\bullet, \bullet)$  is symmetric, we must have  $f(v \otimes u - z \otimes w) = (v, u) - (z, w) = 0$ . As such  $f$  is the zero map on  $\Lambda^2 V$ , so  $f(v \otimes u) = f(z \otimes w)$ , meaning  $(v, u) = (z, w)$  as required.

Similarly if  $(\bullet, \bullet)$  is antisymmetric, then if  $p_2(v \otimes u) = p_2(z \otimes w)$ , then  $v \otimes u - z \otimes w \in \ker p_2 = \text{Sym}^2 V$ . Since  $(\bullet, \bullet)$  is antisymmetric we have  $f(v \otimes u + z \otimes w) = (v, u) + (z, w) = 0$ , so  $f$  is the zero map on  $\text{Sym}^2 V$  and thus  $(v, u) = f(v \otimes u) = f(z \otimes w) = (z, w)$  as required.

## 5 Problem

Let  $G$  be a finite group and  $V$  be an irreducible  $G$ -representation over  $\mathbb{C}$ . Let  $\sigma: \mathbb{C} \rightarrow \mathbb{C}$  denote complex conjugation. Suppose  $V$  admits a nondegenerate invariant bilinear form  $(\bullet, \bullet)$ . Let  $\langle \bullet, \bullet \rangle$  be an invariant inner product (which always exists) on  $V$ .

- (1) Let  $J$  be the composition  $V \rightarrow V^\vee \rightarrow V$  of the function  $v \mapsto (\bullet, v)$  composed with the inverse of  $v \mapsto \langle \bullet, v \rangle$ . Show that  $J$  is  $G$ -equivariant and  $\mathbb{R}$ -linear, but not  $\mathbb{C}$ -linear. Show that  $J^2$  is multiplication by a scalar  $0 \neq \lambda \in \mathbb{C}$ .
- (2) Show that  $J^2 = \lambda \in \mathbb{R}$ , and that if  $(\bullet, \bullet)$  is symmetric then  $\lambda > 0$ , and if it is antisymmetric  $\lambda < 0$ .
- (3) Replacing  $(\bullet, \bullet)$  with  $\frac{1}{\sqrt{|\lambda|}}(\bullet, \bullet)$ , show that we may assume  $\lambda = \pm 1$ .
- (4) Consider  $V$  a real representation, and as such an  $\mathbb{R}[G]$ -module. Show that if  $(\bullet, \bullet)$  is antisymmetric, there is a homomorphism  $\mathbb{H} \rightarrow \text{end}_{\mathbb{R}[G]}(V)$  which sends  $i$  to multiplication by  $i$  and  $j$  to  $J$ .

- (1) Recall that the inverse of  $v \mapsto \langle \bullet, v \rangle$  is  $\phi \mapsto \sum_{i=1}^n \sigma \phi(e_i) e_i$ , where  $\{e_i\}_{i=1}^n$  an orthonormal basis of  $V$ . As such,  $J$  is defined by

$$v \mapsto \sum_{i=1}^n \sigma(e_i, v) e_i$$

Now, let  $g \in G$ , then

$$gv \mapsto \sum_{i=1}^n \sigma(e_i, gv)e_i = \sum_i \sigma(g^{-1}e_i, v)e_i = \sum_i \sigma(e_i, v)ge_i = gJv$$

So  $J$  is indeed  $G$ -equivariant.

Note that

$$J = \sum_{i=1}^n \sigma(e_i, \bullet)e_i$$

so it is the sum of maps of the form  $v \mapsto \sigma(e_i, \bullet)e_i$ . All of which are  $\mathbb{R}$ -linear (since  $(\bullet, \bullet)$  is bilinear and  $\sigma$  is  $\mathbb{R}$ -linear). Thus  $J$  is  $\mathbb{R}$ -linear.

But

$$J(iv) = \sum_j \sigma(e_j, iv)e_i = \sum_j -i\sigma(e_j, v)e_i = -iJ(v)$$

Now, if  $J(v) \neq 0$  then we have  $-iJ(v) \neq iJ(v)$ . Indeed, since the bilinear form is nondegenerate, there is a  $v$  such that  $(e_i, v) \neq 0$ . As such  $Jv \neq 0$  and we have shown that  $J$  is not  $\mathbb{C}$ -linear.

Finally, let us consider  $J^2$ :

$$J^2v = \sum_i \sigma\left(e_i, \sum_j \sigma(e_j, v)e_j\right)e_i = \sum_i \sum_j (e_j, v)\sigma(e_i, e_j)e_i$$

Now, notice that  $J^v$  is  $\mathbb{C}$ -linear. Indeed:

$$J^2(zv) = \sum_{i,j} (e_j, zv)\sigma(e_i, e_j)e_i = z \sum_{i,j} (e_j, v)\sigma(e_i, e_j)e_i = zJ^2v$$

So since  $J^2$  is  $G$ -equivariant,  $J^2 \in \text{end}_G(V) = \mathbb{F} \cdot \text{id}$ , since  $V$  is irreducible.

Now,  $J^2 \neq 0$ . After all, if we focus on  $J^2v$ 's  $i$ th coordinate, it is equal to

$$\sum_j (e_j, v)\sigma(e_i, e_j) = \left( \sum_j \sigma(e_i, e_j)e_j, v \right)$$

Now, since  $\{e_i\}$  forms a basis, we cannot have  $(e_i, e_j) = 0$  (since the bilinear form is nondegenerate). As such the vector  $\sum_j \sigma(e_i, e_j)e_j$  is nonzero. Again by non-degeneracy this means there exists a  $v$  such that  $J^2v \neq 0$ . So indeed we have  $J^2 = \lambda \text{id}$  for  $\lambda \neq 0$ .

(2) Notice that

$$\langle v, Jw \rangle = \left\langle v, \sum_i \sigma(e_i, w)e_i \right\rangle = \sum_i (e_i, w) \langle v, e_i \rangle = (\sum_i \langle v, e_i \rangle e_i, w) = (v, w)$$

And so  $\langle w, Jv \rangle = (w, v)$ . So if  $(v, w) = \epsilon(w, v)$  then  $\langle v, Jw \rangle = \epsilon \langle w, Jv \rangle$ . In particular,

$$\bar{\lambda} \langle v, v \rangle = \langle v, J^2v \rangle = \epsilon \langle Jv, Jv \rangle$$

So let  $v \in V$  where  $Jv \neq 0$ , then we have  $\bar{\lambda}$  must be real and have the same sign as  $\epsilon$ . In particular, if the bilinear form is symmetric,  $\lambda > 0$ , and if it is antisymmetric  $\lambda < 0$ .

- (3) Note that if we replace  $(\bullet, \bullet)$  with  $\alpha(\bullet, \bullet)$  then we scale the map  $v \mapsto (\bullet, v)$  by  $\alpha$ , while the other map doesn't change. In particular, this means that  $J$  is scaled by  $\alpha$  and  $J^2$  by  $\alpha^2$ , i.e.  $J^2 = \alpha^2 \lambda \text{id}$ . Specifically, we can take  $\alpha = 1/\sqrt{|\lambda|}$ , and we get that  $J^2 = \lambda/|\lambda| \text{id}$ , so  $J^2 = \pm \text{id}$ .
- (4) To define a morphism  $f: \mathbb{H} \rightarrow \text{end}_{\mathbb{R}[G]}(V)$ , we define the image on  $i, j$  and extend by linearity and multiplicativity. By the presentation of  $Q_8 \subseteq \mathbb{H}$  (which is  $Q_8 = \langle i, j \mid i^4 = 1, i^2 = j^2, iji = j \rangle$ ), it is sufficient to have  $f(i), f(j)$  satisfy the following relations:

$$f(i)^4 = 1, \quad f(i)^2 = f(j)^2, \quad f(i)f(j)f(i) = f(j)$$

Indeed, since the bilinear form is antisymmetric, we have  $\lambda = -1$  and so  $J^2 = -\text{id}$ . Thus we have

$$i^4 \text{id} = \text{id}, \quad i^2 \text{id} = -\text{id} = J^2, \quad i^2 J = -J \neq J$$

so no such homomorphism can exist.